src/DepList.v
@@ -1,73 +1,9 @@
 Require Import List EqdepClass.
 Require Export EquivDec.
+Require Import Decidables.
 
 Set Implicit Arguments.
-
-Theorem EquivDec_refl_left (T : Type) {c : EqDec T (@eq T)} :
-  forall (n : T), equiv_dec n n = left (refl_equal _).
-Proof.
-  intros. destruct (equiv_dec n n); try congruence.
-  Require Eqdep_dec.
-  rewrite (Eqdep_dec.UIP_dec (A := T) (@equiv_dec _ _ _ c) e (refl_equal _)).
-  reflexivity.
-Qed.
-
-Class SemiDec (t : Type) : Type :=
-{ seq_dec : forall a b : t, option (a = b) }.
-Global Instance EquivDec_SemiDec t (EQ : EqDec t (@eq t)) : SemiDec t :=
-{ seq_dec := fun a b =>
-  match equiv_dec a b with
-    | left pf => Some pf
-    | right _ => None
-  end 
-}.
-
-Global Instance SemiDec_option T (S : SemiDec T) : SemiDec (option T) :=
-{ seq_dec := fun a b =>
-  match a as a, b as b return option (a = b) with
-    | None , None => Some (refl_equal _)
-    | Some x , Some y => 
-      match seq_dec x y with
-        | None => None
-        | Some pf => 
-          match pf in _ = t return option (Some x = Some t) with
-            | refl_equal => Some (refl_equal _)
-          end
-      end
-    | _ , _ => None
-  end
-}.
-
-Global Instance SemiDec_list T (S : SemiDec T) : SemiDec (list T) :=
-{ seq_dec := fix seq_dec' a b : option (a = b) :=
-  match a as a, b as b return option (a = b) with
-    | nil , nil => Some (refl_equal _)
-    | x :: xs , y :: ys => 
-      match seq_dec x y with
-        | None => None
-        | Some pf => 
-          match seq_dec' xs ys with
-            | None => None
-            | Some pf' => 
-              match pf in _ = t , pf' in _ = t' return option (x :: xs = t :: t') with
-                | refl_equal , refl_equal => Some (refl_equal _)
-              end
-          end
-      end
-    | _ , _ => None
-  end
-}.
-
-Inductive dcomp T (a b : T) : Type :=
-| Lt | Gt | Eq : a = b -> dcomp a b.
-
-Class Comparable (t : Type) : Type :=
-{ cmp_dec : forall a b : t, dcomp a b }.
-Class SemiComparable (t : Type) : Type :=
-{ scmp_dec : forall a b : t, option (dcomp a b) }.
-Global Instance Comparable_SemiComparable t (SC : Comparable t) 
-  : SemiComparable t :=
-{ scmp_dec := fun a b => Some (cmp_dec a b) }.
+Set Strict Implicit.
 
 Section fin.
   Variable A : Type.
@@ -709,3 +645,5 @@ Section hlist_fold2.
         hlist_fold2 hr (hlist_tl r) (f acc fr (hlist_hd r))
     end. 
 End hlist_fold2.
+
+Export Decidables.
